@prefix xsd:   <http://www.w3.org/2001/XMLSchema#> .
@prefix owl:   <http://www.w3.org/2002/07/owl#> .
@prefix rdf:   <http://www.w3.org/1999/02/22-rdf-syntax-ns#> .
@prefix rdfs:  <http://www.w3.org/2000/01/rdf-schema#> .
@prefix skos:  <http://www.w3.org/2004/02/skos/core#> .
@prefix dct:   <http://purl.org/dc/terms/> .
@prefix qb:    <http://purl.org/linked-data/cube#> .

@prefix dsapi: <http://www.epimorphics.com/public/vocabulary/dsapi#> .
@prefix :    <http://www.epimorphics.com/public/vocabulary/dsapi#> .

# Simple vocabulary to enable datasets and dsds to be annotated for improved API access

dsapi: a owl:Ontology;
    rdfs:label "DS API"@en;
    rdfs:comment "Vocabulary for configuring Data Services API"@en;
    dct:contributor "Dave Reynolds";
    .
    
# Base level properties for configuring a dataset

:Dataset a owl:Class;
    rdfs:label "Dataset";
    rdfs:comment """Specification for a data set to accessed through the data services API. 
Needs either a qb_dataset or a baseQuery to define the contents of the dataset.
The structure is taken from either the :aspect definitions given here, from directly reference
DSD or implicitly from the DSD associated with the QB dataset.  """@en;
    rdfs:subClassOf [owl:onProperty skos:notation    ; owl:cardinality 1];
    rdfs:subClassOf [owl:onProperty rdfs:label       ; owl:minCardinality 1];
    rdfs:subClassOf [owl:onProperty dct:description  ; owl:minCardinality 0];
    .
    
:qb_dataset a owl:ObjectProperty;
    rdfs:label "qb dataset"@en;
    rdfs:comment "Indicates a Data Cube dataset whose observations are the contents of this dsapi data set"@en;
    rdfs:domain :Dataset;
    rdfs:range  qb:DataSet;
    .
    
:qb_dsd a owl:ObjectProperty;
    rdfs:label "qb dsd"@en;
    rdfs:comment "Indicates a Data Cube DataStructureDefinition defining the aspect structure of the data set."@en;
    rdfs:domain :Dataset;
    rdfs:range  qb:DataStructureDefinition;
    .
    
:baseQuery  a owl:DatatypeProperty;
    rdfs:label "base query"@en;
    rdfs:comment """Gives the textual source of a SPARQL BGP which will bind any member
of the dataset to the ?item variable."""@en;
    rdfs:domain :Dataset;
    rdfs:range  xsd:string
    .    
:aspect a owl:ObjectProperty;
    rdfs:label "aspect"@en;
    rdfs:comment "Indicates a locally-configured 'aspect' of the data set."@en;
    rdfs:domain :Dataset;
    rdfs:range  :Aspect;
    .
    
# Configuration an aspect definition

:Aspect a owl:Class;
    rdfs:label "Aspect";
    rdfs:comment "Specification of a single aspect of the data set"@en;
    rdfs:subClassOf [owl:onProperty skos:notation    ; owl:cardinality 1];
    rdfs:subClassOf [owl:onProperty rdfs:label       ; owl:minCardinality 1];
    rdfs:subClassOf [owl:onProperty dct:description  ; owl:minCardinality 0];
    rdfs:subClassOf [owl:onProperty rdfs:range       ; owl:minCardinality 0];
    rdfs:subClassOf [owl:onProperty :optional        ; owl:minCardinality 0; owl:maxCardinality 1];
    rdfs:subClassOf [owl:onProperty :multivalued     ; owl:minCardinality 0; owl:maxCardinality 1];
    rdfs:subClassOf [owl:onProperty :propertyPath    ; owl:minCardinality 0];
    rdfs:subClassOf [owl:onProperty :rangeConstraint ; owl:minCardinality 0];
    .
    
:optional a owl:DatatypeProperty;
    rdfs:label "optional"@en;
    rdfs:comment "Set to true if the aspect is optional, default is false"@en;
    rdfs:domain :Aspect;
    rdfs:range  xsd:boolean;
    .    
    
:multivalued a owl:DatatypeProperty;
    rdfs:label "multi-valued"@en;
    rdfs:comment "Set to true if the aspect can have multiple values, default is false"@en;
    rdfs:domain :Aspect;
    rdfs:range  xsd:boolean;
    .    
    
:propertyPath a owl:DatatypeProperty;
    rdfs:label "property path"@en;
    rdfs:comment "Source text of a SPARQL property path expression that links a element of the data set to the aspect value."@en;
    rdfs:domain :Aspect;
    rdfs:range  xsd:string;
    .    
    
:rangeConstraint a owl:ObjectProperty;
    rdfs:label "range constraint"@en;
    rdfs:comment "Indicates limits to the range of values which will be present for this aspect."@en;
    rdfs:domain :Aspect;
    rdfs:range  :RangeConstraint;
    .
    
:RangeConstraint  a owl:Class;
    rdfs:label "Range constraint";
    rdfs:comment "Constraint on the range of values which will be present for the corresponding aspect."@en;
    .
 
:lowerBound a owl:DatatypeProperty;
    rdfs:label "lower bound"@en;
    rdfs:comment "Lowest value expected for a measure or other cube component"@en;
    rdfs:domain :RangeConstraint;
    .
    
:upperBound a owl:DatatypeProperty;
    rdfs:label "upper bound"@en;
    rdfs:comment "Highest value expected for a measure or other cube component"@en;
    rdfs:domain :RangeConstraint;
    .
    
